theories/Decidable.v
@@ -17,7 +17,7 @@ Instance show_typ : Show typ :=
 
 Fixpoint show_term' (t : term) :=
   match t with
-  | var n => ("[id " ++ show n ++  "]")%string
+  | var n => ("[" ++ show n ++  "]")%string
   | abs T t => ("(λ : " ++ show T ++". " ++ show_term' t ++ ")")%string
   | app t1 t2 => ("(" ++ show_term' t1 ++ " " ++ show_term' t2 ++ ")")%string
   | tabs T1 t2 => ("(Λ " ++  show T1 ++ ". " ++ show_term' t2 ++ ")")%string
@@ -56,118 +56,299 @@ Instance show_result : Show result :=
   { show := show_result' }.
 
 (** ** Well Formedness *)
-Fixpoint dc_wf_typ (e : env) (T : typ) {struct T} : bool :=
-  match T with
-  | tvar X      => ((get_bound e X) <> None ?)
-  | top         => true
-  | arrow T1 T2 => (dc_wf_typ e T1) && (dc_wf_typ e T2)
-  | all T1 T2   => (dc_wf_typ e T1) && (dc_wf_typ (ebound e T1) T2)
-  end.
+Fixpoint dc_wf_typ (e : env) (T : typ) {struct T} : decidable (wf_typ e T). 
+  refine
+    (match T with
+     | tvar X      => _
+     | top         => left I
+     | arrow T1 T2 => _
+     | all T1 T2   => _
+     end); cbn.
+  - destruct ((get_bound e X)) eqn:Hbound.
+    + left. intros H. inversion H.
+    + right. exact.
+  - destruct (dc_wf_typ e T1). 2: right;intuition.
+    destruct (dc_wf_typ e T2); [left | right]; intuition.
+  - destruct (dc_wf_typ e T1). 2: right;intuition.
+    destruct (dc_wf_typ (ebound e T1) T2); [left | right]; intuition.
+Defined.
 
-Lemma dc_wf_typ_correct (e : env) (T : typ) :
-  wf_typ e T <-> dc_wf_typ e T = true.
-Proof with intuition.
-  split; intro; cbn. 
-  - generalize dependent e.
-    induction T; intros; cbn in *...
-    + destruct (get_bound e n) eqn:E; try congruence. 
-      destruct t... 
-  - generalize dependent e.
-    induction T; intros; cbn in *;
-      try solve [apply andb_prop in H; intuition]. 
-    + destruct (get_bound e n)... destruct t; cbv in H; congruence.
-    + trivial.
-Qed. 
+Fixpoint dc_wf_term (e : env) (t : term) {struct t} : decidable (wf_term e t).
+  destruct t; cbn.
+  - destruct (get_var e n); [left | right].
+    + discriminate.
+    + congruence.
+  - destruct (dc_wf_typ e t). 2:right; intuition.
+    destruct (dc_wf_term (evar e t) t0); [left | right]; intuition.
+  - destruct (dc_wf_term e t1). 2:right; intuition.
+    destruct (dc_wf_term e t2); [left | right]; intuition.
+    Show Proof.
+  - destruct (dc_wf_typ e t). 2:right; intuition.
+    destruct (dc_wf_term (ebound e t) t0); [left | right]; intuition.
+  - destruct (dc_wf_term e t). 2:right; intuition.
+    destruct (dc_wf_typ e t0); [left | right]; intuition.
+Defined.
 
+Fixpoint dc_wf_env (e : env) : decidable (wf_env e).
+  refine
+    (match e with
+     | empty      => left I
+     | evar e T
+     | ebound e T =>
+         _
+     end); cbn.
+  - destruct (dc_wf_typ e T). 2: right; intuition.
+    + destruct (dc_wf_env e); [left | right]; intuition.
+  - destruct (dc_wf_typ e T). 2: right; intuition.
+    + destruct (dc_wf_env e); [left | right]; intuition.
+Defined.
 
-Fixpoint dc_wf_term (e : env) (t : term) {struct t} : bool :=
-  match t with
-  | var x      => get_var e x <> None ?
-  | abs T1 t2  => dc_wf_typ e T1  && dc_wf_term (evar e T1) t2
-  | app t1 t2  => dc_wf_term e t1 && dc_wf_term e t2
-  | tabs T1 t2 => dc_wf_typ e T1  && dc_wf_term (ebound e T1) t2
-  | tapp t1 T2 => dc_wf_term e t1 && dc_wf_typ e T2
-  end.
-
-Hint Resolve -> dc_wf_typ_correct : code.
-Hint Resolve <- dc_wf_typ_correct : code.
-
-Lemma dc_wf_term_correct (e : env) (t : term) :
-  wf_term e t <-> dc_wf_term e t = true.
-Proof with intuition. 
-  split; intros; cbn. 
-  - generalize dependent e.
-    induction t; intros; cbn in *...
-    + destruct (get_var e n) eqn:E; try congruence. 
-      destruct t...
-  - generalize dependent e.
-    induction t; intros; cbn in *;
-      try solve [apply andb_prop in H; intuition]...
-    + destruct (get_var e n)... 
-      destruct t; cbv in H; congruence.
-Qed. 
-
-Fixpoint dc_wf_env (e : env) : bool :=
-  match e with
-    empty      => true
-  | evar e T   => dc_wf_typ e T && dc_wf_env e
-  | ebound e T => dc_wf_typ e T && dc_wf_env e
-  end.
-
-Lemma dc_wf_env_correct (e : env) :
-  wf_env e <-> dc_wf_env e = true.
-Proof with intuition.
-  split; intros.
-  - induction e; cbn in *...
-  - induction e; cbn in *; auto; split; apply andb_prop in H...
-Qed.
-
-(** ** Type Checking *)
-Fixpoint count_tvar (e : env) : nat :=
-  match e with
-  | empty => O
-  | evar e _ => count_tvar e
-  | ebound e _ => S (count_tvar e)
-  end.
-
+(** ** Subtyping *)
 Fixpoint sub_check (e : env) (T1 T2 : typ) (n : nat)
   : @result bool :=
   match n with
   | O => OutOfFuel 
   | S n =>  
       match T1, T2 with
-      | _, top => Result (dc_wf_env e && dc_wf_typ e T1)%bool
-      | tvar X1, tvar X2 =>
-          Result (dc_wf_env e && (X1 = X2 ?) && dc_wf_typ e (tvar X1))%bool
-      | tvar X1, _ =>
-          match get_bound e X1 with
-          | None => Result false 
-          | Some T1' =>
-              sub_check e T1' T2 n
-          end
+      | _, top =>               (** SA_Top *)
+          Result (dc_wf_env e && dc_wf_typ e T1)%bool
+      | tvar X1, _ =>           (** SA_Refl_TVar  *)
+          if (tvar X1 = T2) ?
+          then Result (dc_wf_env e && dc_wf_typ e (tvar X1))%bool
+          else 
+            match get_bound e X1 with
+            | None => Result false 
+            | Some T1' =>
+                sub_check e T1' T2 n
+            end
       | arrow S1 S2, arrow T1 T2 =>
           match sub_check e T1 S1 n with
-          | Result b1 => match sub_check e S2 T2 n with
-                         | Result b2 => Result (b1 && b2)%bool
-                         | _ => OutOfFuel
-                         end
-          | _ => OutOfFuel
+          | Result true => sub_check e S2 T2 n
+          | r => r
           end
       | all S1 S2, all T1 T2 => 
           match sub_check e T1 S1 n with
-          | Result b1 => match sub_check  (ebound e T1) S2 T2 n with
-                       | Result b2 => Result (b1 && b2)%bool
-                       | _ => OutOfFuel
-                       end
-          | _ => OutOfFuel
+          | Result true => sub_check (ebound e T1) S2 T2 n
+          | r => r
           end
       | _, _ => Result false
       end
   end.
 
+(** Convert boolean result equivalence to relation *)
+Ltac invR :=
+  match goal with
+  | [H : Result ?P = Result true |- _] =>
+      let H' := fresh "Hconj" in
+      (destruct P eqn:H' ; try congruence; try (apply andb_prop in H'))
+  | [|- (Result ?P = Result true) -> _] =>
+      let H' := fresh "Hconj" in
+      (destruct P eqn:H'; try congruence; try (apply andb_prop in H'); intros)
+  | [H : Result ?P = Result ?Q |- _] =>
+      (inversion H; clear H; subst)
+  | [|- Result ?P = Result ?Q -> _] =>
+      let H' := fresh "HinvR" in (move=> H'; inversion H'; clear H'; subst)
+  | [|- ?P = Result ?Q -> _] =>
+      let H' := fresh "HinvR" in (destruct P eqn:H'; try exact; try congruence)
+  end.
+
+
+
+Definition reflect_wf_term e t : reflect (wf_term e t) (dc_wf_term e t).
+  apply sumboolP.
+Defined.
+
+Definition reflect_wf_typ e T : reflect (wf_typ e T) (dc_wf_typ e T).
+  apply sumboolP.
+Defined.
+
+Definition reflect_wf_env e : reflect (wf_env e) (dc_wf_env e).
+  apply sumboolP.
+Defined.
+
+Ltac solveWfE :=
+  intuition;
+  match goal with
+  | [ |- (wf_typ ?E ?T)] =>
+      apply (elimT (reflect_wf_typ E T)); auto
+  | [ |- (wf_term ?E ?T)] =>
+      apply (elimT (reflect_wf_term E T)); auto
+  | [ |- (wf_env ?E)] =>
+      apply (elimT (reflect_wf_env E)); auto
+  end.
+
+Ltac solveWfI' :=
+  match goal with
+  | [ |- context [dc_wf_env ?E]] => 
+      rewrite (introT (reflect_wf_env E)); auto
+  | [ |- context[dc_wf_typ ?E ?T]] => 
+      rewrite (introT (reflect_wf_typ E T)); auto
+  | [ |- context[dc_wf_term ?E ?t]] => 
+      rewrite (introT (reflect_wf_term E t)); auto
+  | _ => fail
+  end; repeat solveWfI'.
+  
+Ltac solveWfI :=
+  intuition; solveWfI'.
+
+Theorem sub_check_implies_sub :
+  forall n E T1 T2,
+    sub_check E T1 T2 n = Result true ->
+    sub E T1 T2. 
+Proof with solveWfE.
+  induction n; intros *. cbn; congruence.
+  - destruct T1.
+    unfold sub_check; destruct dec as [Hdec | Hdec].
+    + inversion Hdec; subst. invR; constructor...
+    + fold sub_check.
+      destruct T2; intros;
+        try solve
+            [ destruct (get_bound E n0) eqn:H3;
+              [ rename t into T1; apply SA_Trans_TVar with T1; intuition
+              | congruence ]].
+      invR. constructor...
+    + destruct T2; cbn; try congruence. invR. constructor...
+    + destruct T2 eqn:E2; try solve [cbn; congruence].
+      * unfold sub_check; invR. constructor...
+      * destruct (sub_check E t1 T1_1 n) as [[|]|] eqn:E3; cbn; rewrite E3;
+          try congruence. constructor...
+    + destruct T2 eqn:E2; try solve [cbn; congruence].
+      * unfold sub_check; invR. constructor...
+      * destruct (sub_check E t1 T1_1 n) as [[|]|] eqn:E3; cbn; rewrite E3;
+          try congruence. constructor...
+Qed.        
+
+Ltac solveR f :=
+  match goal with
+  | [ |- context [(f ?x ?y ?z ?a)]] =>
+      let H1 := fresh "Hslv" in
+      (destruct (f x y z a) as [[|]|] eqn:H1;
+       try solve [intros; congruence])
+  | [ |- context [(f ?x ?y ?z)]] =>
+      let H1 := fresh "Hslv" in
+      let T := fresh "T" in
+      (destruct (f x y z) as [[T|]|] eqn:H1;
+       try solve [intros; congruence])
+  | [ |- context [(f ?x ?y)]] =>
+      let H1 := fresh "Hslv" in
+      (destruct (f x y) as [|] eqn:H1;
+       try solve [intros; congruence])
+  | [ |- context [(f ?x)]] =>
+      let H1 := fresh "Hslv" in
+      (destruct (f x) as [|] eqn:H1;
+       try solve [intros; congruence])
+  | _ => fail
+  end.
+
+Lemma sub_check_fuel_widen :
+  forall n1 n2 E T1 T2,
+    n1 <= n2 ->
+    sub_check E T1 T2 n1 = Result true ->
+    sub_check E T1 T2 n2 = Result true.
+Proof.
+  induction n1; intros * Hle. 1: cbn; congruence.
+  destruct n2 as [|n2]. 1: lia.
+  unfold sub_check. fold sub_check.
+  destruct T1; try exact.
+  - destruct T2; try intuition;
+      try solve [destruct dec as [Hdec | Hdec]; try exact;
+                 destruct (get_bound E n); try congruence; intuition].
+  - destruct T2; try intuition.
+    move: H. solveR sub_check. apply (IHn1 n2) in Hslv. 2:lia.
+    intros. rewrite Hslv. apply (IHn1 n2). lia. exact.
+  - destruct T2; try intuition.
+    move: H. solveR sub_check. apply (IHn1 n2) in Hslv. 2:lia.
+    intros. rewrite Hslv. apply (IHn1 n2). lia. exact.
+Qed.
+
+Theorem sub_implies_sub_check :
+  forall E T1 T2,
+    sub E T1 T2 -> 
+    exists n, sub_check E T1 T2 n = Result true. 
+Proof with solveWfI.
+  intros * H. apply sub_wf in H as Hwf. induction H.
+  - exists 1. unfold sub_check. 
+    destruct S...
+  - exists 1. unfold sub_check. destruct dec; try congruence...
+  - apply sub_wf in H0. destruct IHsub as [n' IHsub]; intuition.
+    exists (S n'). unfold sub_check. destruct dec as [Hdec | Hdec].
+    + inversion Hdec; subst... 
+    + fold sub_check. destruct T; try solve [rewrite H; auto]...
+  - intuition. cbn in H3, H4; intuition. 
+    destruct (H2, H5) as [[n1 Hsub1] [n2 Hsub2]].
+    exists (S (n1 + n2)). cbn.
+    apply (sub_check_fuel_widen _ (n1 + n2)) in Hsub1. 2: lia.
+    apply (sub_check_fuel_widen _ (n1 + n2)) in Hsub2. 2: lia.
+    rewrite Hsub1. exact.
+  - apply sub_wf in H0. intuition. cbn in H2, H6. intuition.
+    destruct (H3, H7) as [[n1 Hsub1] [n2 Hsub2]].
+    exists (S (n1 + n2)). cbn.
+    apply (sub_check_fuel_widen _ (n1 + n2)) in Hsub1. 2: lia.
+    apply (sub_check_fuel_widen _ (n1 + n2)) in Hsub2. 2: lia.
+    rewrite Hsub1. exact.
+Qed.
+
+Theorem sub_check_correct :
+  forall e T1 T2,
+    sub e T1 T2 <-> exists n, sub_check e T1 T2 n = Result true.
+Proof.
+  intros. split.
+  - apply sub_implies_sub_check.
+  - intros [n H].  apply sub_check_implies_sub with n. exact.
+Qed.
+
+(** ** Type Checking *)
+Fixpoint promote_tvar (e : env) (T : typ) (fl : nat) : result :=
+  if dc_wf_env e && dc_wf_typ e T then 
+    match T with
+    | tvar n =>
+        match get_bound e n with
+        | Some T =>
+            match fl with
+            | O => OutOfFuel
+            | S fl => promote_tvar e T fl
+            end
+        | _ => Result None
+        end
+    | _ => Result (Some T)
+    end
+  else Result None.
+
+Ltac solveWfR :=
+  match goal with
+  | [ |- context [dc_wf_env ?E]] => 
+      destruct (reflect_wf_env E); auto
+  | [ |- context[dc_wf_typ ?E ?T]] => 
+      destruct (reflect_wf_typ E T); auto
+  | [ |- context[dc_wf_term ?E ?t]] => 
+      destruct (reflect_wf_term E t); auto
+  | _ => fail
+  end; repeat solveWfR.
+
+  
+Lemma promote_tvar_implies_sub :
+  forall fl e T T',
+    promote_tvar e T fl = Result (Some T') -> sub e T T'.
+Proof with (solveWfR; cbn; try congruence).
+  induction fl; intros *.
+  - (* O *)
+    unfold promote_tvar...
+    destruct T; try solve [intros; invR; apply sub_reflexivity; intuition].
+    destruct (get_bound e n); congruence.
+  - (* S fl *)
+    unfold promote_tvar... fold promote_tvar.
+    destruct T; try solve [invR ; apply sub_reflexivity; intuition].
+    destruct (get_bound e n) eqn:Hbound. 2: congruence.
+    intros. apply IHfl in H.
+    apply SA_Trans_TVar with t; intuition.
+Qed.  
+
 Fixpoint get_typ (e : env) (t : term) (fuel : nat) : @result (option typ) :=
   match t with
-  | var x => Result (get_var e x)
+  | var x =>
+      if dc_wf_env e
+      then Result (get_var e x)
+      else Result None
   | abs T1 t2 =>
       match get_typ (evar e T1) t2 fuel with
       | Result (Some T2) => Result (Some (arrow T1 T2))
@@ -175,9 +356,19 @@ Fixpoint get_typ (e : env) (t : term) (fuel : nat) : @result (option typ) :=
       end
   | app t1 t2 =>
       match get_typ e t1 fuel with
-      | Result (Some (arrow T11 T12)) =>
-          match get_typ e t2 fuel with
-          | Result (Some T2) => Result (if T11 = T2 ? then Some T12 else None)
+      | Result (Some T1) =>
+          match promote_tvar e T1 fuel with
+          | Result (Some (arrow T11 T12)) =>
+              match get_typ e t2 fuel with
+              | Result (Some T2) => 
+                  match sub_check e T2 T11 fuel with
+                  | Result true => Result (Some T12)
+                  | Result false => Result None
+                  | _ => OutOfFuel
+                  end
+              | rst => rst
+              end
+          | Result _ => Result None
           | rst => rst
           end
       | rst => rst
@@ -189,16 +380,20 @@ Fixpoint get_typ (e : env) (t : term) (fuel : nat) : @result (option typ) :=
       end
   | tapp t1 T2 => 
       match get_typ e t1 fuel with
-      | Result (Some (all T11 T12)) =>
-          match sub_check e T2 T11 fuel with
-          | Result true => Result (Some (tsubst T12 0 T2))
-          | Result false => Result None
-          | _ => OutOfFuel
+      | Result (Some T1) =>
+          match promote_tvar e T1 fuel with
+          | Result (Some (all T11 T12)) =>
+              match sub_check e T2 T11 fuel with
+              | Result true => Result (Some (tsubst T12 0 T2))
+              | Result false => Result None
+              | _ => OutOfFuel
+              end
+          | Result _ => Result None
+          | rst => rst
           end
       | rst => rst
       end
   end.
-
 
 Definition type_check (e : env) (t : term) (T : typ) (fuel : nat) :
   @result bool :=
@@ -208,25 +403,316 @@ Definition type_check (e : env) (t : term) (T : typ) (fuel : nat) :
   | _ => OutOfFuel
   end.
 
+Hint Resolve sub_check_implies_sub : code. 
 
-(** ** Value *)
-Definition dc_value (t : term) : bool :=
-  match t with
-  | abs _ _  => true
-  | tabs _ _ => true
-  | _        => false
-  end.
-
-Lemma dc_value_implies_value : forall t, dc_value t = true -> value t.
-Proof. intros t. destruct t; cbn; auto. Qed.
-
-Lemma value_implies_dc_value : forall t, value t -> dc_value t = true. 
-Proof. intros t. destruct t; cbn; auto. Qed.
-
-Lemma dc_value_correct (t : term) :
-  dc_value t = true <-> value t.
+Theorem get_typ_implies_typing :
+  forall t e T n, get_typ e t n = Result (Some T) -> typing e t T.
 Proof.
-  split. exact (dc_value_implies_value _). exact (value_implies_dc_value _).
+  induction t; intros *; cbn.
+  - solveWfR. 2:congruence.
+    intros. inversion H. constructor; intuition.
+  - solveR get_typ. invR. constructor. eauto. 
+  - solveR get_typ. rename Hslv into Htyp.
+    solveR promote_tvar. rename Hslv into Htyp0.
+    destruct T1; try congruence.
+    solveR get_typ. rename Hslv into Htyp1.
+    solveR sub_check; intros. invR. rename Hslv into Hsub.
+    (* convert all dec to relations  *)
+    apply promote_tvar_implies_sub in Htyp0.
+    apply sub_check_implies_sub in Hsub. 
+    apply IHt1 in Htyp. apply IHt2 in Htyp1.
+    apply T_App with T1_1.
+    apply T_Sub with T0; exact. 
+    apply T_Sub with T1; exact.
+  - solveR get_typ. invR. constructor. eauto.
+  - solveR get_typ. rename Hslv into Htyp.
+    solveR promote_tvar. rename Hslv into Htyp0.
+    destruct T1; try congruence.
+    solveR sub_check. rename Hslv into Hsub. invR.
+    apply IHt in Htyp. apply promote_tvar_implies_sub in Htyp0.
+    apply sub_check_implies_sub in Hsub.
+    econstructor. 2: exact Hsub. eapply T_Sub. exact Htyp. exact. 
 Qed.
 
+Hint Resolve get_typ_implies_typing : code.
 
+Theorem type_check_implies_typing :
+  forall n t e T, type_check e t T n = Result true -> typing e t T.
+Proof with intuition. 
+  intros *. unfold type_check. solveR get_typ.
+  intros. apply T_Sub with T0.
+  exact (get_typ_implies_typing _ _ _ _ Hslv).
+  exact (sub_check_implies_sub _ _ _ _ H).
+Qed.
+
+Lemma promote_tvar_fuel_widen :
+  forall n1 n2 E T1 T2,
+    n1 <= n2 ->
+    promote_tvar E T1 n1 = Result (Some T2) ->
+    promote_tvar E T1 n2 = Result (Some T2).
+Proof with (solveWfR; cbn; try congruence).
+  induction n1; intros * Hle.
+  - destruct n2. exact.
+    unfold promote_tvar... fold promote_tvar.
+    destruct T1; try exact.
+    destruct (get_bound E n); congruence.
+  - destruct n2. lia.
+    unfold promote_tvar... fold promote_tvar.
+    destruct T1; try exact.
+    destruct (get_bound E n). 2:congruence.
+    intuition.
+Qed.
+Hint Rewrite sub_check_fuel_widen : code.
+
+Ltac solveRe f H n1 n2 :=
+  solveR f; 
+  match goal with 
+  | [ Htyp : _ |- _ ] =>
+      apply (H n1 n2) in Htyp; try lia; rewrite Htyp; clear Htyp
+  | [ Hsub : _ |- _ ] =>
+      apply (H n1 n2) in Hsub; try lia; rewrite Hsub; clear Hsub
+  end.
+
+Lemma get_typ_fuel_widen :
+  forall t n1 n2 E T,
+    n1 <= n2 ->
+    get_typ E t n1 = Result (Some T) ->
+    get_typ E t n2 = Result (Some T).
+Proof.
+  induction t; intros * Hle. 
+  - exact.
+  - cbn. solveR get_typ. invR.
+    apply (IHt _ n2) in Hslv. 2: lia.
+    rewrite Hslv. exact.
+  - cbn.
+    solveRe get_typ IHt1 n1 n2.
+    solveRe promote_tvar promote_tvar_fuel_widen n1 n2.
+    destruct T1; try congruence.
+    solveRe get_typ IHt2 n1 n2.
+    solveRe sub_check sub_check_fuel_widen n1 n2.
+    exact.
+  - destruct n1, n2. 1:exact. 2:lia.
+    + cbn. solveRe get_typ IHt 0 (S n2). exact.
+    + cbn. solveRe get_typ IHt (S n1) (S n2). exact.
+  - destruct n1, n2. 1:exact. 2:lia.
+    + unfold get_typ. fold get_typ.
+      solveRe get_typ IHt 0 (S n2).
+      solveRe promote_tvar promote_tvar_fuel_widen 0 (S n2).
+      case T1; exact.
+    + unfold get_typ. fold get_typ.
+      solveRe get_typ IHt (S n1) (S n2).
+      solveRe promote_tvar promote_tvar_fuel_widen (S n1) (S n2).
+      case T1; try exact. intros *.
+      solveRe sub_check sub_check_fuel_widen (S n1) (S n2).
+      exact.
+Qed.
+
+Ltac solve_left n T :=
+  exists n, T; split; [(try exact; try apply sub_reflexivity); intuition | idtac].
+
+Ltac appWS H :=
+      let Hsub' := fresh "Hsub" in
+      let HwfE := fresh "HwfE" in
+      let HwfT := fresh "HwfT" in
+      let HwfU := fresh "HwfU'" in
+      pose proof H as Hsub';
+      apply sub_wf in Hsub' as [HwfE [HwfT HwfU]]
+. 
+
+Ltac appWT H :=
+  let Htyp' := fresh "Htyp" in
+  let HwfE := fresh "HwfE" in
+  let Hwft := fresh "Hwft" in
+  let HwfU := fresh "HwfU'" in
+  pose proof H as Htyp';
+  apply typing_wf in Htyp' as [HwfE [Hwft HwfU]]
+.
+
+Ltac step H :=
+  unfold H; fold H.
+
+Lemma sub_arrow_implies_promote_tvar_arrow :
+  forall e T1 T21 T22,
+    sub e T1 (arrow T21 T22) -> exists fl T31 T32,
+      promote_tvar e T1 fl = Result (Some (arrow T31 T32)) /\
+        sub e T21 T31 /\ sub e T32 T22.
+Proof with (solveWfI; cbn).
+  intros * Hsub. appWS Hsub. 
+  remember (arrow T21 T22) as Tarrow.
+  dependent induction Hsub; inversion HeqTarrow; clear HeqTarrow; subst.
+  - appWS Hsub. 
+    destruct IHHsub as [fl [T41 [T42 [Hprom [Hsub1 Hsub2]]]]]; try exact.
+    exists (S fl), T41, T42. split. 2: exact.
+    step promote_tvar... rewrite H. exact.
+  - exists 0, S1, S2. step promote_tvar... 
+Qed.
+
+Lemma sub_all_implies_promote_tvar_all :
+  forall e T1 T21 T22,
+    sub e T1 (all T21 T22) -> exists fl T31 T32,
+      promote_tvar e T1 fl = Result (Some (all T31 T32)) /\
+        sub e T21 T31 /\ sub (ebound e T21) T32 T22.
+Proof with (solveWfI; cbn).
+  intros * Hsub. appWS Hsub. 
+  remember (all T21 T22) as Tarrow.
+  dependent induction Hsub; inversion HeqTarrow; clear HeqTarrow; subst.
+  - appWS Hsub. 
+    destruct IHHsub as [fl [T41 [T42 [Hprom [Hsub1 Hsub2]]]]]; try exact.
+    exists (S fl), T41, T42. split. 2: exact.
+    step promote_tvar... rewrite H. exact.
+  - exists 0, S1, S2. step promote_tvar... 
+Qed.
+
+Theorem typing_implies_get_typ :
+  forall t e T,
+    typing e t T ->
+    exists n T', sub e T' T /\ get_typ e t n = Result (Some T').
+Proof.
+  intros * H. appWT H. induction H.
+  - (* T_Var *)
+    solve_left 1 T. cbn. solveWfI. f_equal. exact.
+  - (* T_Abs *)
+    appWT H. destruct IHtyping as [n [T [Hsub Htyp]]]; intuition.
+    exists n, (arrow T1 T). cbn in HwfU'.
+    split. 2: cbn; rewrite Htyp; reflexivity.
+    constructor.
+    + apply sub_reflexivity. exact. intuition.
+    + replace (sub e T T2) with (sub (remove_var (evar e T1) 0) T T2)
+        by reflexivity.
+      apply sub_strengthening_var. exact.
+  - (* T_App *)
+    appWT H. appWT H0.
+    (** construct all fuels  *)
+    destruct IHtyping1 as [n1 [T1 [Hsub1 Htyp1]]]; try solve [intuition].
+    destruct IHtyping2 as [n2 [T2 [Hsub2 Htyp2]]]; try solve [intuition].
+    destruct (sub_arrow_implies_promote_tvar_arrow e T1 T11 T12) as
+      [n11 [T11' [T12' [Hprom1 [Hpsub1 Hpsub2]]]]]. { exact. }
+    destruct (sub_implies_sub_check e T2 T11') as [n3 Hsub3].
+    { apply sub_transitivity with T11; exact. }
+    (** clear up environment *)
+    clear HwfE1 HwfE0.
+    pose (n1 + n2 + n11 + n3) as n. solve_left (S n) T12'.
+    (** rewrite *)
+    step get_typ. 
+    apply (get_typ_fuel_widen _ _ (S n)) in Htyp1. 2:lia. rewrite Htyp1.
+    apply (promote_tvar_fuel_widen n11 (S n)) in Hprom1. 2:lia. rewrite Hprom1.
+    apply (get_typ_fuel_widen _ _ (S n)) in Htyp2. 2:lia. rewrite Htyp2.
+    apply (sub_check_fuel_widen _ (S n)) in Hsub3. 2:lia. rewrite Hsub3.
+    reflexivity.
+  - (* T_Tabs *)
+    appWT H.
+    destruct IHtyping as [n [T2' [Hsub Htyp]]]; intuition.
+    cbn in HwfU'.
+    exists n, (all T1 T2').
+    split. { constructor. 2:exact. apply sub_reflexivity; intuition. }
+    cbn. rewrite Htyp. reflexivity. 
+  - (* T_Tapp *)
+    appWT H.
+    (** construct all fuels  *)
+    destruct IHtyping as [n1 [T1 [Hsub1 Htyp1]]]; intuition.
+    destruct (sub_all_implies_promote_tvar_all e T1 T11 T12) as
+      [n2 [T11' [T12' [Hprom1 [Hpsub1 Hpsub2]]]]]. { exact. }
+    destruct (sub_implies_sub_check e T2 T11') as [n3 Hsub3].
+    { apply sub_transitivity with T11; exact. }
+    pose (n1 + n2 + n3) as n. exists (S n),  (tsubst T12' 0 T2).
+    split. { apply tsubst_preserves_subtyping with (ebound e T11).
+             constructor. exact. exact. }
+    step get_typ.
+    rewrite (get_typ_fuel_widen _ _ (S n) _ _ _ Htyp1). 2:lia.
+    apply (promote_tvar_fuel_widen n2 (S n)) in Hprom1. 2:lia. rewrite Hprom1.
+    apply (sub_check_fuel_widen _ (S n)) in Hsub3. 2:lia. rewrite Hsub3.
+    reflexivity.
+  - appWT H. 
+    destruct IHtyping as [n1 [U [Hsub1 Htyp1]]]; intuition.
+    exists n1, U. split. { apply sub_transitivity with T1; exact. } exact.
+Qed.
+
+Theorem typing_implies_type_check :
+  forall t e T, typing e t T -> exists n, type_check e t T n = Result true.
+Proof. 
+  intros * H. 
+  destruct (typing_implies_get_typ t e T) as [n1 [U [Hsub Htyp]]]; intuition.
+  destruct (sub_implies_sub_check e U T) as [n2 Hsub2]. 1:exact.
+  pose (n1 + n2) as n. exists (S n). unfold type_check.
+  rewrite (get_typ_fuel_widen _ _ (S n) _ _ _ Htyp). 2:lia.
+  rewrite (sub_check_fuel_widen _ (S n) _ _ _ _ Hsub2). 2:lia.
+  reflexivity.
+Qed.    
+
+Theorem type_check_correct :
+  forall t e T,
+    typing e t T <-> exists n, type_check e t T n = Result true.
+Proof.
+  intros; split.
+  - apply typing_implies_type_check.
+  - intros [n H]. apply type_check_implies_typing with n. exact.
+Qed.
+
+(** * Q: What's the Tactics for fold -> unfold? *)
+(** ** Value *)
+Definition dc_value t : decidable (value t).
+  refine
+    (match t with 
+     | abs _ _  => left I
+     | tabs _ _ => left I
+     | _        => right id
+     end).
+Defined.
+
+Theorem reflect_value : forall t, reflect (value t) (dc_value t).
+  intros; destruct t; cbn; try solve[right; elim]; try solve[left; apply I].
+Qed.
+
+Ltac solveVE :=
+  intuition;
+  match goal with
+  | [ |- (value ?v)] =>
+      apply (elimT (reflect_value v)); auto
+  end.
+
+Ltac solveVI :=
+  match goal with
+  | [ |- context [value ?v]] => 
+      rewrite (introT (reflect_value v)); auto
+  end.
+
+Ltac solveVR :=
+  match goal with
+  | [ |- context [dc_value ?v]] => 
+      destruct (reflect_value v); auto
+  end.
+
+(** ** Shorthands : unwrap unnecessary fuels *)
+Definition type_check' :=
+  fun E t T =>
+    match type_check E t T 100 with
+    | Result true => true
+    | _ => false
+    end. 
+
+Definition get_typ' :=
+  fun E t =>
+    match get_typ E t 100 with
+    | Result o => o
+    | _ => None
+    end. 
+
+Definition sub_check' :=
+  fun e T1 T2 => match sub_check e T1 T2 100 with
+                 | Result true => true
+                 | _ => false
+                 end.
+
+Fixpoint count_tvar (e : env) : nat :=
+  match e with
+  | empty => O
+  | evar e _ => count_tvar e
+  | ebound e _ => S (count_tvar e)
+  end.
+
+Fixpoint count_var (E : env) : nat :=
+  match E with
+  | empty => 0
+  | evar E _ => S (count_var E)
+  | ebound E _ => (count_var E)
+  end.
