theories/Example.v
@@ -94,3 +94,159 @@ Sample (gen_exact_typ0
              top)). 
 
 
+(*  *)
+
+Example ex_sub1_typ :=
+  (all top
+       (arrow (tvar 0)
+              (all top 
+                   (arrow (tvar 0)
+                          (all (arrow (tvar 0) (tvar 1))
+                               (arrow (tvar 0)
+                                      (all (tvar 0)
+                                           (arrow (tvar 0)
+                                                  (arrow (tvar 2) (tvar 3)))))))))). 
+
+Eval cbv in show ex_sub1_typ.
+
+
+Fixpoint get_env (t : term) : env :=
+  match t with
+  | abs T t => evar (get_env t) T
+  | tabs T t => ebound (get_env t) T
+  | _ => empty
+  end.
+
+Example ex_sub1_tc :=
+  (fun x =>
+     (tabs top
+           (abs (tvar 0)
+                (tabs top 
+                      (abs (tvar 0)
+                           (tabs (arrow (tvar 0) (tvar 1))
+                                 (abs (tvar 0)
+                                      (tabs (tvar 0)
+                                            (abs (tvar 0) x))))))))).
+
+(** [gen_sub_term 0 empty ex_sub1_typ] 
+    is capable of generating all 3 following variants *)
+Sample (gen_sub_term 0 empty ex_sub1_typ).
+
+Example ex_sub1_t1 :=
+  ex_sub1_tc (var 0).
+
+Example ex_sub1_t2 :=
+  ex_sub1_tc (var 1).
+
+Example ex_sub1_t3 :=
+  ex_sub1_tc (abs (tvar 2) (var 4)).
+
+Eval cbv in type_check empty ex_sub1_t3 ex_sub1_typ 100.
+Eval cbv in type_check empty ex_sub1_t2 ex_sub1_typ 100.
+Eval cbv in type_check empty ex_sub1_t1 ex_sub1_typ 100.
+
+(** {∀{∀Top . (<0> -> <0>)} . (<0> -> <0>)} *)
+Example ex_t1 :=
+  all (all top (arrow (tvar 0) (tvar 0))) (arrow (tvar 0) (tvar 0)). 
+
+(** {∀Top . (<0> -> <0>)} *)
+Example ex_t2 :=
+  (all top (arrow (tvar 0) (tvar 0))). 
+
+
+(** [t2] <: [t1] *)
+Eval cbv in sub_check' empty ex_t2 ex_t1.
+
+(** test [get_typ]
+    ((λ : {∀{∀Top . (<0> -> <0>)} . (<0> -> <0>)}.
+      (Λ {∀Top . (<0> -> <0>)}. (λ : <0>. [id 0])))
+     (Λ Top. (λ : <0>. [id 0]))) 
+*)
+Example ex_tm1 :=
+  tabs top (abs (tvar 0) (var 0)).
+
+Eval cbv in get_typ empty ex_tm1 10.
+
+Example ex_tm2 :=
+  tabs (all top (arrow (tvar 0) (tvar 0))) (abs (tvar 0) (var 0)).
+
+Eval cbv in get_typ empty ex_tm2 10.
+
+Example ex_tm3 :=
+  app (abs ex_t1 ex_tm2) ex_tm1.
+
+Eval cbv in (get_typ empty (abs ex_t1 ex_tm2) 10).
+
+Eval cbv in get_typ empty ex_tm3 10.
+
+(** ** More Subtype Examples *)
+Example ex_sub2_ty1 :=
+  all top (arrow (tvar 0) (tvar 0)). 
+Example ex_sub2_ty2 :=
+  all (all top (arrow (tvar 0) (tvar 0))) (arrow (tvar 0) (tvar 0)). 
+
+Eval cbv in sub_check' empty ex_sub2_ty1 ex_sub2_ty2. 
+(* 
+Eval cbv in sub_check' empty
+                       (arrow ex_sub2_ty2 ex_sub2_ty2)
+                       (arrow ex_sub2_ty1 ex_sub2_ty1).
+ *)
+
+(** ** Subsitution Related Examples *)
+Definition ex_subst_sub t := all top (all top t).
+
+Example ex_subst_ty1 :=
+  ex_subst_sub
+    (arrow (tvar 0) (arrow (tvar 1) (arrow (tvar 1) (tvar 0)))).
+
+Sample (gen_exact_term (measure_max_typ ex_subst_ty1) empty ex_subst_ty1).
+
+Example ex_subst_tm1 :=
+  let f1 t := tabs top (tabs top t) in
+  let f2 t := (abs (tvar 0) (abs (tvar 1) t)) in
+  let t3 := (app (abs (tvar 0) (abs (tvar 1) (var 3))) (var 1)) in
+  f1 (f2 t3).
+
+Example id_est1 : (G (option term)) :=
+  ret ex_subst_tm1.
+Example id_esty1 : (G (option typ)) :=
+  ret ex_subst_ty1.
+
+Eval cbv in get_typ' empty ex_subst_tm1.
+Eval cbv in type_check' empty ex_subst_tm1 ex_subst_ty1.
+
+
+Example ty2 :=
+  all (all top top) (all (tvar 0) (all (tvar 1) top)). 
+
+Example ty2' :=
+  (all (tvar 0) (all (tvar 1) top)).
+
+Eval cbv in fetch_candidate_typs ty2'.
+
+
+Example sub1 :
+  sub empty
+      (all top (all (all (tvar 0) (tvar 1)) top))
+      (all top (all (all (tvar 0) (tvar 0)) top)). 
+Proof with intuition.
+  constructor. constructor... cbn; apply I.
+  constructor.
+  - constructor. constructor... cbn...
+    eapply SA_Trans_TVar; cbn...
+    apply SA_Refl_TVar... cbn... congruence.
+  - constructor... cbn... congruence. congruence.
+Qed.
+
+Example sub2 :
+  sub empty
+      (all top (all (tvar 0) (arrow (tvar 1) (tvar 1))))
+      (all top (all (tvar 0) (arrow (tvar 0) (tvar 1)))).
+Proof with easy.
+  constructor. constructor...
+  constructor. constructor...
+  constructor.
+  eapply SA_Trans_TVar. cbn. reflexivity.
+  apply SA_Refl_TVar...
+  constructor... 
+Qed.
