theories/Generator.v
@@ -3,12 +3,7 @@ From FSUB Require Import FSub.
 From FSUB Require Import Decidable.
 From FSUB Require Import Reduction.
 
-Fixpoint count_var (E : env) : nat :=
-  match E with
-  | empty => 0
-  | evar E _ => S (count_var E)
-  | ebound E _ => (count_var E)
-  end.
+(** * Generator: System F<: Random Generators *)
 
 Fixpoint tlift (T : typ) (m : nat) :=
   match m with
@@ -17,13 +12,6 @@ Fixpoint tlift (T : typ) (m : nat) :=
   end.
 
 (** ** Generate (Almost) SystemF *)
-Definition gen_top_comb (g : G (option typ)) : G (option typ) := 
-  a <- g ;;
-  match a with
-  | Some T => returnGen a
-  | None => returnGen (Some top)
-  end.
-
 Definition gen_exact_tvar0' (E : env) : list (G typ) :=
   match count_tvar E with
   | O => []
@@ -66,12 +54,12 @@ Fixpoint gen_exact_typ (n : nat) (E : env) : G (option typ) :=
   | S n =>
       let gen_all :=
         T1 <- oneOf [ret top;   (* allow top in TVar *)
-                     gen_exact_typ (pred (pred n)) E] ;;
+                     gen_exact_typ n E] ;;
         T2 <- gen_exact_typ n (ebound E T1) ;;
         ret (all T1 T2) in
       let gen_arrow :=
-        T1 <- oneOf_ (gen_exact_typ (pred (pred n)) E)
-                     ((gen_exact_typ (pred (pred n)) E)
+        T1 <- oneOf_ (gen_exact_typ n E)
+                     ((gen_exact_typ n E)
                         :: (map (fmap Some) (gen_exact_tvar0' E)));;
         T2 <- gen_exact_typ n (evar E T1) ;;
         ret (arrow T1 T2) in
@@ -79,7 +67,22 @@ Fixpoint gen_exact_typ (n : nat) (E : env) : G (option typ) :=
       backtrack [(5, gen_arrow) ; (5, gen_all) ; (1, gen_exact_typ0 E)]
   end.
 
-Sample (gen_exact_typ 3 empty).
+(*
+Definition fetch_tvar_typs (E : env) :=
+  let ntvar := count_tvar E in
+  let fix f n :=
+    match n with
+    | O => []
+    | S n =>
+        match get_bound E n with
+        | Some T => [T]
+        | None => []
+        end ++ (f n)
+    end in
+  f ntvar.
+*)
+   
+
 
 Fixpoint get_bound_vars (T : typ) (n m : nat) (E : env) : list term :=
   match E with
@@ -138,16 +141,14 @@ Fixpoint gen_exact_term (n : nat) (E : env) (T : typ) : G (option term) :=
         end in
       (** Generate App *)
       let g2 :=
-        T1 <- gen_exact_typ (pred n) E;; (* include more context aware generation? *)
-        (* t1 <- gen_exact_term n (evar E T1) T;; *)
-        t1 <- gen_exact_term (pred n) E (arrow T1 T);;
+        T1 <- gen_exact_typ n E;;
+        t1 <- gen_exact_term n E (arrow T1 T);;
         t2 <- gen_exact_term n E T1;;
-        (* returnGen (Some (app (abs T1 t1) t2)) *)
         returnGen (Some (app t1 t2))
       in
       (** Generate TApp *)
       let g3 :=
-        T1 <- gen_exact_typ (pred n) E;; 
+        T1 <- gen_exact_typ n E;; 
         t1 <- gen_exact_term n E (all T1 (tshift 0 T));;
         returnGen (Some (tapp t1 T1))
       in backtrack [(1, g0); (1, g1); (1, g2); (1, g3)]
@@ -158,19 +159,14 @@ Definition gen_exact (n : nat) : G (option term) :=
   T <- gen_exact_typ n empty;;
   gen_exact_term n empty T.
 
-Sample (gen_exact 5).
+(* Sample (gen_exact 5). *)
 
-Definition type_check' :=
-  fun E t T => type_check E t T 100. 
-Definition get_typ' :=
-  fun E t => get_typ E t 100. 
 
 (** ** Generate Subtype *)
-Definition sub_check' :=
-  fun e T1 T2 => sub_check e T1 T2 20. 
 
-(* TODO : Abstraction *)
-Definition gen_sub_tvar' (E : env) (T2 : typ) : list typ :=
+(** Find out super or sub type of the given [typ] in the environment *)
+Definition find_sub_tvar  
+           (E : env) (T2 : typ) : list typ :=
   let n := count_tvar E in
   let fix f n1 :=
     match n1 with
@@ -180,19 +176,18 @@ Definition gen_sub_tvar' (E : env) (T2 : typ) : list typ :=
         | None => []
         | Some T1 => 
             let T' := match sub_check' E T1 T2 with
-                      | Result true => [T1]
+                      | true => [T1]
                       | _ => []
                       end in
             T' ++ (f n1)
         end
     end in
   f n.
-
-
+  
 Definition gen_sub_tvar (E : env) (T2 : typ) : G typ :=
-  elems_ T2 (gen_sub_tvar' E T2). 
+  elems_ T2 (find_sub_tvar E T2). 
 
-Definition gen_sup_tvar' (E : env) (n1 : nat) : list typ :=
+Definition find_sup_tvar (E : env) (n1 : nat) : list typ :=
   match get_bound E n1 with
   | None => []
   | Some T1 => 
@@ -205,7 +200,7 @@ Definition gen_sup_tvar' (E : env) (n1 : nat) : list typ :=
             | None => []
             | Some T2 => 
                 let T' := match sub_check' E T1 T2 with
-                          | Result true => [tvar n1]
+                          | true => [tvar n1]
                           | _ => []
                           end in
                 T' ++ (f n2)
@@ -214,9 +209,8 @@ Definition gen_sup_tvar' (E : env) (n1 : nat) : list typ :=
       f n
   end.
 
-
 Definition gen_sup_tvar (E : env) (n1 : nat) : G typ :=
-  elems_ (tvar n1) (gen_sup_tvar' E n1). 
+  elems_ (tvar n1) (find_sup_tvar E n1). 
 
 Fixpoint gen_sub_typ (n : nat) (E : env) (T : typ) : G typ :=
   match n with
@@ -234,8 +228,8 @@ Fixpoint gen_sub_typ (n : nat) (E : env) (T : typ) : G typ :=
         | tvar n => ret (tvar n)
         | arrow T1 T2 =>
             (** [S1] :> [T1] -> 
-              [S2] <: [T2] ->
-              arrow [S1] [S2] <: arrow [T1] [T2] 
+                [S2] <: [T2] ->
+                arrow [S1] [S2] <: arrow [T1] [T2] 
              *)
             S1 <- gen_sup_typ n E T1;;
             S2 <- gen_sub_typ n E T2;;
@@ -245,7 +239,7 @@ Fixpoint gen_sub_typ (n : nat) (E : env) (T : typ) : G typ :=
             S2 <- gen_sub_typ n (ebound E T1) T2;;
             ret (all S1 S2)
         end in
-      let g2 := map ret (gen_sub_tvar' E T) in
+      let g2 := map ret (find_sub_tvar E T) in
       oneOf_ (ret T) ((ret T) :: g1 :: g2)
   end
 with
@@ -270,24 +264,274 @@ gen_sup_typ (n : nat) (E : env) (T : typ) : G typ :=
   end
 .
 
-(** ** Generate SystemF Sub *)
-(** Idea0: Fixpoint iteration *)
-
-Fixpoint multistep {A}
-           (n : nat)
-           (step : A -> option A)
-           (t : A)
-           (is_value : A -> bool) : @result (bool * A) :=
-  match n with
-  | O => OutOfFuel
-  | S n =>
-      match step t with
-      | Some t => multistep n step t is_value
-      | None => Result ((is_value t), t)
-      end
+Definition c_gen_sub_typ g n E : G (option typ) :=
+  oT <- (g n E) ;;
+  match oT with
+  | None => ret None 
+  | Some T => liftM Some (gen_sub_typ n E T)
   end.
 
-(** TODO : More Type-Parameter-Aware Term Generation
+Definition c_gen_sup_typ g n E : G (option typ) :=
+  oT <- (g n E) ;;
+  match oT with
+  | None => ret None 
+  | Some T => liftM Some (gen_sup_typ n E T)
+  end.
+
+      
+(** ** Generate System F <:
     
-    Λ<:top. λ<:<0>. <: (<0> -> <0>). λ <:<0>. [0] [1]
- *)
+    - Generate a type to be used as the super type of the program
+    - Widen the type of an exact type step by step
+*)
+
+(** Generate a [typ] *)
+(** Reworked [gen_typ] : allow bare [top]s and [arrow]s *)
+Definition fetch_var_typs (E : env) : list typ :=
+  let nvar := count_var E in
+  let fix f n :=
+    match n with
+    | O => []
+    | S n =>
+        match get_var E n with
+        | Some T => [T]
+        | None => []
+        end ++ (f n)
+    end in
+  f nvar.
+
+
+
+(** for each [var] in the env, "upcasts" can be done to it *)
+Definition fetch_good_typs (E : env) : list typ :=
+  let vars := fetch_var_typs E in
+  let ntvars :=  count_tvar E in
+  let fix f n :=
+    match n with
+    | O => []
+    | S n => (tvar n) :: f n
+    end in
+  let tvars := f ntvars in 
+  List.fold_right
+    (fun v acc =>
+       acc ++ match v with
+              | tvar n =>
+                  v ::          (** bound var itself *)
+                    match get_bound E n with
+                    | Some T => (** upcasts to its super type *)
+                        List.filter (sub_check' E T) tvars
+                    | None => []
+                    end
+              (** More can be done here: analyze structure of the typ *)
+              | _ => [v]
+              end)
+    [] vars.
+    
+(** Motivation: 
+
+    ∀ top. ∀ <0>. ∀ <0>. <0> -> ◻ *)
+Example env_with_sub :=
+  (evar
+     (ebound
+        (ebound
+           (ebound empty
+                   top)
+           (tvar 0))
+        (tvar 1))
+     (tvar 0)). 
+
+Eval cbv in fetch_var_typs env_with_sub. 
+Eval cbv in fetch_good_typs env_with_sub. 
+
+Definition gen_typ0 (E : env) (r : bool) : G typ := 
+  if r
+  then                          (** Restricted: must be sub bound [var] *)
+    freq [(1, ret top);
+          let Ts := fetch_good_typs E in
+          (List.length Ts, elems_ top Ts)]
+  else                          (** Any bound [var] or [tvar] suffice *)
+    freq [(1, ret top);
+          let n'' := count_tvar E in
+          (n'', n' <- choose(0, n'');; ret (tvar n'));
+          let vs := fetch_var_typs E in
+          (List.length vs, elems_ top vs)].
+
+Fixpoint gen_typ (n : nat) (E : env) (r : bool) {struct n} : G typ :=
+  match n with
+  | O =>
+      gen_typ0 E r
+  | S n =>
+      freq [(1, gen_typ0 E r) ;
+            (1, T1 <- gen_typ (n - 1) E false ;;
+                T2 <- gen_typ n (ebound E T1) r ;;
+                ret (all T1 T2)) ; 
+            (1, T1 <- gen_typ (n - 1) E false ;;
+                T2 <- gen_typ n (evar E T1) r ;;
+                ret (arrow T1 T2))]
+  end.
+
+Sample (gen_typ 4 empty true).
+
+Definition gen_opt_typ (n : nat) (E : env) (r : bool) : G (option typ) :=
+  fmap Some (gen_typ n E r).
+
+(** Generate a [term] *)
+
+(** Find a bound var that is of a subtype of [T]  *)
+Fixpoint get_bound_sub_vars (T : typ) (E : env) : list term :=
+  let n := count_var E in
+  let fix f n1 :=
+    match n1 with
+    | O => []
+    | S n1 => 
+        match get_var E n1 with
+        | None => []
+        | Some T1 => 
+            let T' := match sub_check' E T1 T with
+                      | true => [var n1]
+                      | _ => []
+                      end in
+            T' ++ (f n1)
+        end
+    end in
+  f n.
+
+Fixpoint get_bound_sup_vars (T : typ) (E : env) : list term :=
+  let n := count_var E in
+  let fix f n1 :=
+    match n1 with
+    | O => []
+    | S n1 => 
+        match get_var E n1 with
+        | None => []
+        | Some T1 => 
+            let T' := match sub_check' E T T1 with
+                      | true => [var n1]
+                      | _ => []
+                      end in
+            T' ++ (f n1)
+        end
+    end in
+  f n.
+
+Definition gen_bound_sub_vars T E : G (option term) :=
+  elems_ None (map Some (get_bound_sub_vars T E)).
+
+Definition gen_bound_sup_vars T E : G (option term) :=
+  elems_ None (map Some (get_bound_sup_vars T E)).
+
+
+Fixpoint gen_sub_term0 (E : env) (T : typ) : G (option term) :=
+  let g : (G (option term)) :=
+    match T with
+    | arrow T1 T2 =>
+        liftM (abs T1) (gen_sub_term0 (evar E T1) T2)
+    | all T1 T2 =>
+        liftM (tabs T1)
+              (gen_sub_term0 (ebound E T1) T2)
+    | _ => ret None
+    end
+  in     
+  backtrack [(1, g); (1, (gen_bound_sub_vars T E))].
+
+Fixpoint gen_sup_term0 (E : env) (T : typ) : G (option term) :=
+  let g : (G (option term)) :=
+    match T with
+    | arrow T1 T2 =>
+        liftM (abs T1) (gen_sup_term0 (evar E T1) T2)
+    | all T1 T2 =>
+        liftM (tabs T1)
+              (gen_sup_term0 (ebound E T1) T2)
+    | _ => ret None
+    end
+  in     
+  backtrack [(1, g); (1, (gen_bound_sup_vars T E))].
+
+
+(** generate operands to functions in the context *)
+Definition michalsub (E : env) (T : typ) : list typ :=
+  let n := count_var E in
+  let fix f2 T' :=
+    match T' with
+    | arrow T1 T2 =>
+        (** don't need to shift type here: no intro of tvar *)
+        match sub_check' E T2 T with
+        | true => [T1]
+        | _ => []
+        end ++ f2 T2
+    | _ => []
+    end in
+  let fix f n1 :=
+    match n1 with
+    | O => []
+    | S n1 => 
+        match get_var E n1 with
+        | Some T' => f2 T'
+        | None => []
+        end ++ f n1
+    end in
+  f n.
+
+(** not useful? *)
+Definition c_michalsub (g : G (option typ)) (E : env) (T : typ)
+  : G (option typ) :=
+  oneOf_ g (g :: (map (fun x => ret (Some x)) (michalsub E T))).
+
+
+(** Generate a term of a subtype of [T] *)
+Fixpoint gen_sub_term (n : nat) (E : env) (T : typ) : G (option term) :=
+  match n with
+  | O => gen_sub_term0 E T
+  | S n =>
+      let n' := n - 2 in (* n - n / 2 in *)
+      (** Base Case *)
+      let g0 := gen_sub_term0 E T in
+      (** Generate by typ *)
+      let g1 := 
+        match T with
+        | arrow T1 T2 =>
+            T1' <- (c_gen_sup_typ (fun _ _ => ret T1) n E) ;;
+            t2 <- (gen_sub_term n (evar E T1') T2) ;;
+            ret (abs T1' t2)
+        | all T1 T2 =>
+            T1' <- (c_gen_sup_typ (fun _ _ => ret T1) n E) ;;
+            t2 <- (gen_sub_term n (ebound E T1') T2) ;;
+            ret (tabs T1' t2)
+        | _ => g0
+        end in
+      (** Generate App *)
+      let g2 :=
+        (** restricted: to generate the operand term *)
+        T1 <- c_michalsub (gen_opt_typ n' E true) E T;;
+        (** generate [t1] of a subtype of [T1 -> T] *)
+        t1 <- gen_sub_term n' E (arrow T1 T);;
+        (** generate [t2] of a subtype of [T1] *)
+        t2 <- gen_sub_term n' E T1;;
+        returnGen (Some (app t1 t2))
+      in
+      (** Generate TApp : [t1'] is [(tabs T1 t1) T2] <: [T] *)
+      let g3 :=
+        (** unrestricted: typ can be any *)
+        T1 <- gen_opt_typ n' E false;; 
+        T2 <- c_gen_sub_typ (fun _ _ => ret T1) n' E;;
+        t1' <- gen_sub_term n' E (all T1 (tshift 0 T)) ;;
+        returnGen (Some (tapp t1' T2))
+      in backtrack [(1, g0); (1, g1); (1, g2); (1, g3)]
+  end
+.
+
+Sample (gen_opt_typ 2 empty true).
+
+Sample (gen_sub_term 3 empty top).
+
+Definition max_dec n m : nat :=
+  if le_gt_dec n m then m else n.
+
+Fixpoint measure_max_typ (T : typ) : nat :=
+  match T with
+  | tvar _ => 1 
+  | top => 1
+  | arrow T1 T2 => 1 + max_dec (measure_max_typ T1) (measure_max_typ T2)
+  | all T1 T2 => 1 + max_dec (measure_max_typ T1) (measure_max_typ T2)
+  end.
+
