theories/Reduction.v
@@ -1,107 +1,81 @@
-From FSUB Require Import QCLibs.
-From FSUB Require Import FSub.
-From FSUB Require Import Decidable.
+From FSUB Require Import
+     QCLibs
+     FSub
+     Decidable.
+(** * Reduction: Semantics *)
 
-(** ** Computable Reduction Semantics *)
-Program Definition ctx_inj (t : term) : option (ctx * term) :=
+(** ** Alternative Semantics
+    
+    The equivalence between reduction relation and its computable function is
+    hard to prove. 
+
+ *)         
+Fixpoint step' (t : term) : option term :=
+  let appfun' t1 t2 :=
+    t1' <- step' t1;; ret (app t1' t2) in 
+
+  let apparg' t1 t2 :=
+    t2' <- step' t2;; ret (app t1 t2') in
+
+  let typefun' t1 T2 :=
+    t1' <- step' t1;; ret (tapp t1' T2) in 
+
   match t with
   | app t1 t2 =>
-      match dc_value t1 with
-        true => Some (@c_apparg t1 _ c_hole, t2)
-      | false => Some (c_appfun c_hole t2, t1)
+      match t1 with
+      |  abs t11 t12 => 
+           if dc_value t2 
+           then ret (subst t12 0 t2) (* appabs *)
+           else apparg' t1 t2
+      | _ =>
+          if dc_value t1
+          then apparg' t1 t2
+          else appfun' t1 t2
       end
   | tapp t1 T2 =>
-      Some (c_typefun c_hole T2,  t1)
+      match t1 with
+      | tabs t11 T12 => ret (subst_typ T12 0 T2)
+      | _ => typefun' t1 T2            
+      end
   | _ => None
   end.
-Next Obligation.
-  apply dc_value_implies_value. auto.
-Qed.
-Solve All Obligations with easy.
 
-Eval cbn in (ctx_inj (tapp (var 0) top)).
-
-Fixpoint measure_term (t : term) : nat :=
-  match t with
-  | var _ => 1 
-  | abs _ t' => 1 + measure_term t'
-  | app t1 t2 => 1 + measure_term t1 + measure_term t2
-  | tabs _ t2 => 1 + measure_term t2
-  | tapp t1 _ => 1 + measure_term t1
-  end.
-
-Lemma measure_term_le_ctx_inj : forall c t t',
-    Some (c, t') = ctx_inj t -> measure_term t' < measure_term t.
+Lemma red'_not_value :
+  forall t1 t2, red' t1 t2 -> ~ value t1.
 Proof.
-  intros until t. destruct t; intros; cbn in *; try congruence. 
-  - destruct t1; cbn in *; inversion H; clear H; subst; cbn; lia.
-  - inversion H; clear H; subst; lia. 
+  intros * Hred Hcontra.
+  destruct t1; cbn in Hcontra; intuition; inversion Hred.
 Qed.
 
-Program Fixpoint step (t : term) {measure (measure_term t)} : option term :=
-  match t with
-  | app (abs _ t12) t2 =>
-      if dc_value t2 then Some (subst t12 0 t2) else
-        match ctx_inj t with
-        | None => None
-        | Some (c', t') => 
-            match step t' with
-            | Some t'' => Some (ctx_app c' t'')
-            | None => None
-            end
-        end         
-  | tapp (tabs T11 t12) T2 => Some (subst_typ t12 0 T2)
-  | _ => match ctx_inj t with
-         | None => None
-         | Some (c', t') => 
-             match step t' with
-             | Some t'' => Some (ctx_app c' t'')
-             | None => None
-             end
-         end 
-  end.
-Next Obligation.
-  cbn; lia.
-Qed.
-Next Obligation.
-  eapply measure_term_le_ctx_inj. eauto.
-Qed.
-Solve All Obligations with easy.
-
-Compute (step (app
-                 (abs top (var 0))
-                 (abs top (var 0)))).
-Compute (step (abs top (var 0))).
-
-(* Require Extraction. *)
-(* Extraction "step.ml" step. *)
-
-Lemma step_app_value : forall T t1 t2,
-    dc_value t2 = true -> step (app (abs T t1) t2) = Some (subst t1 0 t2).
+Lemma red'_implies_step' :
+  forall t1 t2, red' t1 t2 -> step' t1 = Some t2.
 Proof.
-Admitted.  
-
-(** ** Equivalence in Reduction Semantics *)
-Lemma step_is_red : forall t t', step t = Some t' -> red t t'.
-Proof with intuition. 
-  induction t; intros t'; simpl; intros.
-  - cbn in H; congruence.
-  - cbn in H; congruence.
-  - destruct t1.
-    + cbn in H. congruence.
-    + destruct (dc_value t2) eqn:Et2.
-      * pose proof Et2 as Et2'.
-        apply dc_value_implies_value in Et2.
-        rewrite step_app_value in H. inversion H; subst. constructor.
-        assumption.
-        assumption.
-Admitted.
-
-Lemma red_is_step : forall t t', red t t' -> step t = Some t'.
-Admitted.
-    
-Lemma red_iff_step : forall t t', red t t' <-> step t = Some t'.
-Proof.
-  split. apply red_is_step. apply step_is_red.
+  intros * H; induction H; cbn.
+  - solveVI.
+  - reflexivity.
+  - rewrite IHred'.
+    destruct t1; try solve [inversion IHred']; solveVR; inversion v.
+  - rewrite IHred'. destruct t1; try solve[solveVI].
+    apply red'_not_value in H0.
+    destruct (reflect_value t2); [congruence | reflexivity].
+  - rewrite IHred'.
+    destruct t1; try reflexivity.
+    apply red'_not_value in H.
+    cut (value (tabs t t1)); [congruence | exact].
 Qed.
 
+Lemma step'_implies_red' :
+  forall t1 t2, step' t1 = Some t2 -> red' t1 t2.
+Proof.
+  intros t1.
+  induction t1; intros *; try solve[inv0]; cbn;
+    [destruct t1_1 | destruct t1]; try solveVR;
+    try solve[solveR step'; inv0; constructor; cbn ; intuition];
+    try solve[inv0; constructor; auto].
+Qed.
+
+Theorem step'_correct :
+  forall t1 t2, step' t1 = Some t2 <-> red' t1 t2.
+Proof.
+  intros. split; [apply step'_implies_red' | apply red'_implies_step'].
+Qed. 
