theories/GeneratorSub.v
@@ -1,0 +1,441 @@
+From FSUB Require Import QCLibs.
+From FSUB Require Import FSub.
+From FSUB Require Import Decidable.
+From FSUB Require Import Reduction.
+
+(** * Generator: System F<: Random Generators *)
+
+(** ** Utilities *)
+(** Shorthands : only care about true or false. *)
+Definition type_check' :=
+  fun E t T =>
+    match type_check E t T 100 with
+    | Result true => true
+    | _ => false
+    end. 
+
+Definition get_typ' :=
+  fun E t =>
+    match get_typ E t 100 with
+    | Result o => o
+    | _ => None
+    end. 
+
+Definition sub_check' :=
+  fun e T1 T2 => match sub_check e T1 T2 100 with
+                 | Result true => true
+                 | _ => false
+                 end.
+
+
+Fixpoint count_tvar (e : env) : nat :=
+  match e with
+  | empty => O
+  | evar e _ => count_tvar e
+  | ebound e _ => S (count_tvar e)
+  end.
+
+Fixpoint count_var (E : env) : nat :=
+  match E with
+  | empty => 0
+  | evar E _ => S (count_var E)
+  | ebound E _ => (count_var E)
+  end.
+
+(** ** Generate System F <:
+    
+    - Generate a type to be used as the super type of the program
+    - Narrow the type down to exact subtype terms for termination
+*)
+
+(** *** Generate [typ] *)
+
+(** collect all bound var typs *)
+Definition fetch_var_typs (E : env) : list typ :=
+  let nvar := count_var E in
+  let fix f n :=
+    match n with
+    | O => []
+    | S n =>
+        match get_var E n with
+        | Some T => [T]
+        | None => []
+        end ++ (f n)
+    end in
+  f nvar.
+
+(** collect super bound var types 
+    - for each [var] in the env, perform "upcast" to it 
+ *)
+Definition fetch_good_typs (E : env) : list typ :=
+  let vars := fetch_var_typs E in
+  let ntvars :=  count_tvar E in
+  let fix f n :=
+    match n with
+    | O => []
+    | S n => (tvar n) :: f n
+    end in
+  let tvars := f ntvars in 
+  List.fold_right
+    (fun v acc =>
+       acc ++ match v with
+              | tvar n =>
+                  v ::          (** bound var itself *)
+                    match get_bound E n with
+                    | Some T => (** upcast to its super *)
+                        List.filter (sub_check' E T) tvars
+                    | None => []
+                    end
+              (** More can be done here: analyze structure of the typ *)
+              | _ => [v]
+              end)
+    [] vars.
+    
+(** Motivation: 
+
+    ∀ top. ∀ <0>. ∀ <0>. <0> -> ◻ *)
+Example env_with_sub :=
+  (evar
+     (ebound
+        (ebound
+           (ebound empty
+                   top)
+           (tvar 0))
+        (tvar 1))
+     (tvar 0)). 
+
+Eval cbv in fetch_var_typs env_with_sub. 
+Eval cbv in fetch_good_typs env_with_sub. 
+
+(** Reworked [gen_typ] : allow bare [top]s and [arrow]s *)
+Definition gen_typ0 (E : env) (r : bool) : G typ := 
+  if r
+  then                          (** Restricted: must be sub bound [var] *)
+    freq [(1, ret top);
+          let Ts := fetch_good_typs E in
+          (List.length Ts, elems_ top Ts)]
+  else                          (** Any bound [var] or [tvar] suffice *)
+    freq [(1, ret top);
+          let n'' := count_tvar E in
+          (n'', n' <- choose(0, n'' - 1);; ret (tvar n'));
+          let vs := fetch_var_typs E in
+          (List.length vs, elems_ top vs)].
+
+Fixpoint gen_typ (n : nat) (E : env) (r : bool) {struct n} : G typ :=
+  match n with
+  | O =>
+      gen_typ0 E r
+  | S n =>
+      freq [(1, gen_typ0 E r) ;
+            (1, T1 <- gen_typ (n - 1) E false ;;
+                T2 <- gen_typ n (ebound E T1) r ;;
+                ret (all T1 T2)) ; 
+            (1, T1 <- gen_typ (n - 1) E false ;;
+                T2 <- gen_typ n (evar E T1) r ;;
+                ret (arrow T1 T2))]
+  end.
+
+Sample (gen_typ 4 empty true).
+
+Definition gen_opt_typ (n : nat) (E : env) (r : bool) : G (option typ) :=
+  fmap Some (gen_typ n E r).
+
+Definition find_sub_var_typs (E : env) (T : typ) : list typ :=
+  List.filter (fun T' => sub_check' E T' T) (fetch_var_typs E). 
+
+Definition find_sup_var_typs (E : env) (T : typ) : list typ :=
+  List.filter (sub_check' E T) (fetch_var_typs E). 
+
+Definition find_sub_tvar_typs (E : env) (T : typ) : list typ :=
+  let ntvars :=  count_tvar E in
+  let fix f n :=
+    match n with
+    | O => []
+    | S n => n :: f n
+    end in
+  map tvar
+      (List.filter
+         (fun n =>
+            match get_bound E n with
+            | Some T' => sub_check' E T' T
+            | _ => false
+            end)
+         (f ntvars)).
+
+Fixpoint gen_sub_typ (n : nat) (E : env) (T : typ) {struct n} : G typ :=
+  match n with
+  | O => ret T                  (** [sub] is reflexive *)
+  | S n =>
+      let g1 :=
+        match T with
+        | top =>                
+            gen_typ n E true
+        | tvar n => ret (tvar n)
+        | arrow T1 T2 => 
+            S1 <- gen_sup_typ n E T1;;
+            S2 <- gen_sub_typ n E T2;;
+            ret (arrow S1 S2)
+        | all T1 T2 =>
+            S1 <- gen_sup_typ n E T1;;
+            S2 <- gen_sub_typ n (ebound E T1) T2;;
+            ret (all S1 S2)
+        end in
+      let g2 :=
+        elems_ T ((find_sub_var_typs E T) ++ (find_sub_tvar_typs E T)) in
+      let g2' := T <- g2 ;; gen_sub_typ n E T in
+      oneOf [ret T; g1; g2']
+  end
+with
+gen_sup_typ (n : nat) (E : env) (T : typ) {struct n} : G typ :=
+  match n with
+  | O => ret T                  (** [sup] is reflexive *)
+  | S n =>
+      let g1 :=
+        match T with
+        | top => ret top        (** [top] is the top *)
+        | tvar n' =>
+            match get_bound E n' with
+            | Some T => gen_sup_typ n E T
+            | _ => ret (tvar n')
+            end
+        | arrow T1 T2 =>
+            S1 <- gen_sub_typ n E T1;;
+            S2 <- gen_sup_typ n E T2;;
+            ret (arrow S1 S2)
+        | all T1 T2 =>
+            S1 <- gen_sub_typ n E T1;;
+            S2 <- gen_sup_typ n (ebound E T1) T2;;
+            ret (all S1 S2)
+        end in
+      let g2 := elems_ top (find_sup_var_typs E T) in
+      let g2' := T <- g2 ;; gen_sup_typ n E T in 
+      oneOf [ret T; g1; g2']
+  end
+.
+
+Definition gen_opt_sub_typ (n : nat) (E : env) (T : typ) : G (option typ) :=
+  fmap Some (gen_sub_typ n E T).
+
+Definition gen_opt_sup_typ (n : nat) (E : env) (T : typ) : G (option typ) :=
+  fmap Some (gen_sup_typ n E T).
+
+(** Generate a [term] *)
+(** Fetch bound vars that are <: [T]  *)
+Definition fetch_sub_vars (E : env) (T : typ) : list term :=
+  let n := count_var E in
+  let fix f n1 :=
+    match n1 with
+    | O => []
+    | S n1 => 
+        match get_var E n1 with
+        | None => []
+        | Some T1 => 
+            let T' := match sub_check' E T1 T with
+                      | true => [var n1]
+                      | _ => []
+                      end in
+            T' ++ (f n1)
+        end
+    end in
+  f n.
+
+Definition gen_sub_vars E T : G (option term) :=
+  elems_ None (map Some (fetch_sub_vars E T)).
+
+(** generate operands to functions in the context *)
+Definition michalsub (E : env) (T : typ) : list typ :=
+  let n := count_var E in
+  let fix f2 T' :=
+    match T' with
+    | arrow T1 T2 =>
+        (** don't need to shift type here: no intro of tvar *)
+        match f2 T2 with
+        | [] => if sub_check' E T2 T then [T1] else []
+        | rst => T1 :: rst
+        end
+    | _ => []
+    end in
+  let fix f n1 :=
+    match n1 with
+    | O => []
+    | S n1 => 
+        match get_var E n1 with
+        | Some T' => f2 T'
+        | None => []
+        end ++ f n1
+    end in
+  f n.
+
+(** not useful? *)
+Definition c_michalsub (g : G (option typ)) (E : env) (T : typ)
+  : G (option typ) :=
+  oneOf_ g (g :: (map (fun x => ret (Some x)) (michalsub E T))).
+
+(** Replace free/constant [typ's] in [t] with a new [typ] *)
+
+(** fetch_candidate_typs : 
+    list of free/constant [typ] in [T] under the context [E] 
+ *)
+Definition fetch_candidate_typs (T : typ) : list typ :=
+  let fix fetch_p T n :=
+    match T with
+    | top => true
+    | tvar n' => (** Check if it's free *)
+        n <=? n'
+    | arrow T1 T2 =>
+        ((fetch_p T1 n) && (fetch_p T2 n))%bool
+    | all T1 T2 =>
+        (** not precise here *)
+        ((fetch_p T1 n) && (fetch_p T2 (S n)))%bool
+    end in
+  let fix tunshift T n :=
+    match T with
+    | top => top
+    | tvar n' => tvar (n' - n)
+    | arrow T1 T2 => arrow (tunshift T1 n) (tunshift T2 n)
+    | all T1 T2 => all (tunshift T1 n) (tunshift T2 (S n))
+    end
+  in
+  let fix f T nbound :=
+    (if fetch_p T nbound then [tunshift T nbound] else [])
+      ++
+      (match T with
+       | arrow T1 T2 =>
+           (f T1 nbound) ++ (f T2 nbound)
+       | all T1 T2 =>
+           (f T1 nbound) ++ (f T2 (S nbound))
+       | _ => []
+       end) in
+  f T 0.  
+
+Definition gen_cand (T : typ) : G (option typ) :=
+  elems_ None (map Some (fetch_candidate_typs T)).
+
+(** 2 strategies here: 
+    - [replace_typ T T' n] :
+      replace part of type [T] equal to T'  with [tvar n]
+      (without considering sub)
+    - [mutate_typ E T] :
+      replace part of type [T] by consulting bound types in [E] 
+      (considerng sub typing)
+
+    Which one is better?
+ *)
+
+
+Fixpoint replace_typ T T' n : G typ :=
+  (** more likely to generate replacement *)
+  let g1 := (if T = T' ? then [(3, ret (tvar n))] else [(1, ret T)])  in
+  let g2 :=
+    match T with
+    | arrow T1 T2 =>
+        T1' <- replace_typ T1 T' n ;;
+        T2' <- replace_typ T2 T' n ;;
+        ret (arrow T1' T2')
+    | all T1 T2 => 
+        T1' <- replace_typ T1 T' n ;;
+        T2' <- replace_typ T2 (tshift 0 T') (S n) ;;
+        ret (all T1' T2')
+    | _ => ret T
+    end in
+   freq_ (ret T) ((2, g2) :: g1).
+
+Definition gen_replace T : G (option (typ * typ)) :=
+  oT1 <- gen_cand T ;;
+  match oT1 with
+  | Some T1 =>
+    T2 <- replace_typ (tshift 0 T) (tshift 0 T1) 0 ;;
+    (ret (Some (T1, T2)))
+  | None => ret None
+  end. 
+
+
+Example repl_ty :=
+  (arrow (tvar 0) (arrow (tvar 1) (all top (arrow (tvar 1) (tvar 0))))).
+
+Sample (gen_replace repl_ty).
+
+Fixpoint gen_sub_term0 (E : env) (T : typ) : G (option term) :=
+  let g : (G (option term)) :=
+    match T with
+    | arrow T1 T2 =>
+        liftM (abs T1) (gen_sub_term0 (evar E T1) T2)
+    | all T1 T2 =>
+        liftM (tabs T1)
+              (gen_sub_term0 (ebound E T1) T2)
+    | tvar n =>                 (** guarded by [gen_typ] *)
+        gen_sub_vars E T
+    | top => ret (abs top (var 0)) (** random stuff *)
+    end
+  in     
+  backtrack [(1, g); (1, (gen_sub_vars E T))].
+
+
+(** Generate a term of a subtype of [T] *)
+Fixpoint gen_sub_term (n : nat) (E : env) (T : typ) : G (option term) :=
+  match n with
+  | O => gen_sub_term0 E T
+  | S n =>
+      (* let n' := n - 2 in (* n - n / 2 in *) *)
+      (** Mutate the type based on bound [typ]'s *)
+      
+      let n' := n in
+      (** Base Case *)
+      let g0 := gen_sub_term0 E T in
+      (** Generate by typ *)
+      let g1 := 
+        match T with
+        | arrow T1 T2 =>
+            T1' <- gen_opt_sup_typ n E T1 ;;
+            t2 <- gen_sub_term n (evar E T1') T2 ;;
+            ret (abs T1' t2)
+        | all T1 T2 =>
+            T1' <- gen_opt_sup_typ n E T1 ;;
+            t2 <- gen_sub_term n (ebound E T1') T2 ;;
+            ret (tabs T1' t2)
+        | _ => g0
+        end in
+      (** Generate App *)
+      let g2 :=
+        (** restricted: to generate the operand term *)
+        T1 <- c_michalsub (gen_opt_typ n' E true) E T;;
+        (** generate [t1] of a subtype of [T1 -> T] *)
+        t1 <- gen_sub_term n' E (arrow T1 T);;
+        (** generate [t2] of a subtype of [T1] *)
+        t2 <- gen_sub_term n' E T1;;
+        returnGen (Some (app t1 t2))
+      in
+      (** Generate TApp : [t1'] is [(tabs T1 t1) T2] <: [T] *)
+      let g3 :=
+        (** unrestricted: typ can be any *)
+        T1 <- gen_opt_typ n' E false;; 
+        T2 <- gen_opt_sub_typ n' E T1;;
+        t1' <- gen_sub_term n' E (all T1 (tshift 0 T)) ;;
+        returnGen (Some (tapp t1' T2))
+      in
+      let g4 :=
+        (** unrestricted: typ can be any *)
+        '(T2, T12) <- gen_replace T ;;
+        T11 <- gen_opt_sup_typ n' E T2 ;;
+        t1' <- gen_sub_term n' E (all T11 T12) ;;
+        returnGen (Some (tapp t1' T2))
+      in
+      (** introduce more [app] and  [tapp] at beginning *)
+      backtrack [(1, g0); (1, g1); (n', g2); (n', g3); (n', g4)]
+  end
+.
+
+(*
+Definition max_dec n m : nat :=
+  if le_gt_dec n m then m else n.
+
+Fixpoint measure_max_typ (T : typ) : nat :=
+  match T with
+  | tvar _ => 1 
+  | top => 1
+  | arrow T1 T2 => 1 + max_dec (measure_max_typ T1) (measure_max_typ T2)
+  | all T1 T2 => 1 + max_dec (measure_max_typ T1) (measure_max_typ T2)
+  end.
+
+
+*)
