theories/MutantInterface.v
@@ -1,0 +1,276 @@
+From FSUB Require Import
+     QCLibs
+     FSub
+     Decidable.
+
+(** * Mutant: Bug Injection and Reduction Strategies *)
+
+(** ** Mutants *)
+Inductive Mutant :=
+| NoMutant
+(** [tshift] bugs *)
+| TShiftTVarAll
+| TShiftTVarNoIncr
+| TShiftAllNoIncr
+(** [shift] bugs *)
+| ShiftVarAll
+| ShiftVarNoIncr
+| ShiftAbsNoIncr
+(** [shift_typ] bugs *)
+| ShiftTypTAbsNoIncr
+(** [tsubst] bugs *)
+| TSubstTVarFlip
+| TSubstTVarNoShift
+| TSubstTVarOverShift
+| TSubstAllNoTShift  
+(** [subst] bugs *)
+| SubstVarFlip
+| SubstVarNoDecr
+| SubstAbsNoShift
+| SubstAbsNoIncr
+| SubstTAbsNoShift
+(** [subst_typ] bugs *)
+| SubstTypTAbsNoIncr
+| SubstTypTAbsNoShift
+(** [get_bound] bugs *)
+(** [get_var] bugs *)
+.
+
+Instance dec_eq_Mutant (m1 m2 : Mutant) : Dec (m1 = m2).
+Proof. dec_eq. Defined.
+
+Fixpoint mut {A} (c : Mutant) (x : A)
+                 (my : list (Mutant * A)) : A :=
+  match my with
+  | [] => x
+  | (m,y) :: my' => if c = m? then y else mut c x my'
+  end.
+
+
+(** ** Bug Injection *)
+Fixpoint tshift' (c : Mutant) (X : nat) (T : typ) {struct T} : typ :=
+  let tshift := tshift' c in 
+  match T with
+  | tvar Y      => mut c (tvar (if le_gt_dec X Y then 1 + Y else Y))
+                       [(TShiftTVarAll, tvar (1 + Y));
+                        (TShiftTVarNoIncr, tvar Y)]
+  | top         => top
+  | arrow T1 T2 => arrow (tshift X T1) (tshift X T2)
+  | all T1 T2   => mut c (all (tshift X T1) (tshift (1 + X) T2))
+                       [(TShiftAllNoIncr, all (tshift X T1) (tshift X T2))]
+  end.
+
+Fixpoint shift' (c : Mutant) (x : nat) (t : term) {struct t} : term :=
+  let shift := shift' c in
+  match t with
+  | var y      => mut c (var (if le_gt_dec x y then 1 + y else y))
+                      [(ShiftVarAll, var (1 + y));
+                       (ShiftVarNoIncr, var y)]
+  | abs T1 t2  => mut c (abs T1 (shift (1 + x) t2))
+                      [(ShiftAbsNoIncr, (abs T1 (shift x t2)))]
+  | app t1 t2  => app (shift x t1) (shift x t2)
+  | tabs T1 t2 => tabs T1 (shift x t2)
+  | tapp t1 T2 => tapp (shift x t1) T2
+  end.
+
+Fixpoint shift_typ' (c : Mutant) (X : nat) (t : term) {struct t} : term :=
+  let shift_typ := shift_typ' c in 
+  let tshift := tshift' c in 
+  match t with
+  | var y      => var y
+  | abs T1 t2  => abs (tshift X T1) (shift_typ X t2)
+  | app t1 t2  => app (shift_typ X t1) (shift_typ X t2)
+  | tabs T1 t2 => mut c (tabs (tshift X T1) (shift_typ (1 + X) t2))
+                      [(ShiftTypTAbsNoIncr, tabs (tshift X T1)
+                                                 (shift_typ X t2))]
+  | tapp t1 T2 => tapp (shift_typ X t1) (tshift X T2)
+  end.
+
+Fixpoint tsubst' (c : Mutant) (T : typ) (X : nat) (T' : typ) {struct T} : typ :=
+  let tsubst := tsubst' c in
+  let tshift := tshift' c in
+  match T with
+  | tvar Y =>
+      mut c 
+          (match lt_eq_lt_dec Y X with
+           | inleft (left _)  => tvar Y
+           | inleft (right _) => T'
+           | inright _        => tvar (Y - 1)
+           end)
+          [(TSubstTVarFlip,
+             (match lt_eq_lt_dec Y X with
+              | inleft (left _)  => tvar (Y - 1)
+              | inleft (right _) => T'
+              | inright _        => tvar Y
+              end));
+           (TSubstTVarNoShift,
+             (match lt_eq_lt_dec Y X with
+              | inleft (left _)  => tvar Y
+              | inleft (right _) => T'
+              | inright _        => tvar Y
+              end));
+           (TSubstTVarOverShift,
+             (match lt_eq_lt_dec Y X with
+              | inleft (left _)  => tvar (Y - 1)
+              | inleft (right _) => T'
+              | inright _        => tvar (Y - 1)
+              end))]
+  | top         => top
+  | arrow T1 T2 => arrow (tsubst T1 X T') (tsubst T2 X T')
+  | all T1 T2   =>
+      mut c
+          (all (tsubst T1 X T') (tsubst T2 (1 + X) (tshift 0 T')))
+          [(TSubstAllNoTShift,
+             all (tsubst T1 X T') (tsubst T2 (1 + X) T'))]
+  end.
+
+Fixpoint subst' (c : Mutant) (t : term) (x : nat) (t' : term) {struct t} : term :=
+  let subst := subst' c in
+  let shift := shift' c in
+  let shift_typ := shift_typ' c in
+  match t with
+  | var y =>
+      mut c 
+          (match lt_eq_lt_dec y x with
+           (* x > y : does not affect *)
+           | inleft (left _)  => var y 
+           (* x = y : target for substitution *)
+           | inleft (right _) => t'    
+           (* x < y : var disappears, shift by 1 *)
+           | inright _        => var (y - 1)
+           end)
+          [(SubstVarFlip,
+             (match lt_eq_lt_dec y x with
+              | inleft (left _)  => var (y - 1) 
+              | inleft (right _) => t'    
+              | inright _        => var y
+              end));
+           (SubstVarNoDecr,
+             (match lt_eq_lt_dec y x with
+              | inleft (left _)  => var y 
+              | inleft (right _) => t'    
+              | inright _        => var y
+              end))]
+  | abs T1 t2  =>
+      mut c 
+          (abs T1 (subst t2 (1 + x) (shift 0 t')))
+          [(SubstAbsNoShift, abs T1 (subst t2 (1 + x) t'));
+           (SubstAbsNoIncr, (abs T1 (subst t2 x (shift 0 t'))))]
+  | app t1 t2  => app (subst t1 x t') (subst t2 x t')
+  | tabs T1 t2 =>
+      mut c
+          (tabs T1 (subst t2 x (shift_typ 0 t')))
+          [(SubstTAbsNoShift, (tabs T1 (subst t2 x t')))]
+  | tapp t1 T2 => tapp (subst t1 x t') T2
+  end.
+
+Fixpoint subst_typ' (c : Mutant) (t : term) (X : nat) (T : typ) {struct t} :
+  term :=
+  let subst_typ := subst_typ' c in
+  let subst := subst' c in
+  let tshift := tshift' c in
+  let tsubst := tsubst' c in
+  match t with
+  | var y      => var y
+  | abs T1 t2  => abs (tsubst T1 X T) (subst_typ t2 X T)
+  | app e1 e2  => app (subst_typ e1 X T) (subst_typ e2 X T)
+  | tabs T1 e1 =>
+      mut c
+          (tabs (tsubst T1 X T) (subst_typ e1 (1 + X) (tshift 0 T)))
+          [(SubstTypTAbsNoIncr,
+             tabs (tsubst T1 X T) (subst_typ e1 X (tshift 0 T)));
+           (SubstTypTAbsNoShift,
+             tabs (tsubst T1 X T) (subst_typ e1 (1 + X) T))]
+  | tapp e1 T2 => tapp (subst_typ e1 X T) (tsubst T2 X T)
+  end.
+
+(** ** Mutated Reduction *)
+(** TODO : use [Section] *)
+(** *** Alternative Smallstep Semantics *)
+Fixpoint step'' (m : Mutant) (t : term) : option term :=
+  let step' := step'' m in
+  let subst := subst' m in 
+  let subst_typ := subst_typ' m in 
+  
+  let appfun' t1 t2 :=
+    t1' <- step' t1;; ret (app t1' t2) in 
+
+  let apparg' t1 t2 :=
+    t2' <- step' t2;; ret (app t1 t2') in
+
+  let typefun' t1 T2 :=
+    t1' <- step' t1;; ret (tapp t1' T2) in 
+
+  match t with
+  | app t1 t2 =>
+      match t1 with
+      |  abs t11 t12 => 
+           if dc_value t2 
+           then ret (subst t12 0 t2) (* appabs *)
+           else apparg' t1 t2
+      | _ =>
+          if dc_value t1
+          then apparg' t1 t2
+          else appfun' t1 t2
+      end
+  | tapp t1 T2 =>
+      match t1 with
+      | tabs t11 T12 => ret (subst_typ T12 0 T2)
+      | _ => typefun' t1 T2            
+      end
+  | _ => None
+  end.
+
+
+(** *** Parallel Reduction 
+    Support reduction to normal form.
+ *)
+Fixpoint pstep' (m : Mutant) (t : term) : option term :=
+  let pstep := pstep' m in
+  let subst := subst' m in 
+  let subst_typ := subst_typ' m in 
+  match t with
+  | var _ => ret t 
+  | abs T t =>  liftM (abs T) (pstep t)
+  | app t1 t2 =>
+      match t1 with
+      | abs _ t1 => ret (subst t1 0 t2)
+      | _ => liftM2 app (pstep t1) (pstep t2)
+      end
+  | tabs T t => liftM (tabs T) (pstep t)
+  | tapp t T =>
+      match t with
+      | tabs _ t => ret (subst_typ t 0 T)
+      | _ => liftM (fun t => tapp t T) (pstep t)
+      end
+  end.
+
+Fixpoint is_nf (t : term) :=
+  match t with
+  | var _ => true
+  | abs _ t => is_nf t
+  | app (abs _ _) t2 => false
+  | app t1 t2 => is_nf t1 && is_nf t2
+  | tabs _ t => is_nf t
+  | tapp (tabs _ _) _ => false
+  | tapp t _ => is_nf t
+  end.
+
+
+(** *** Multistep Closure *)
+Fixpoint multistep' {A}
+         (m : Mutant)
+         (n : nat)
+         (step : Mutant -> A -> option A)
+         (t : A)
+         (is_value : A -> bool) : @result (bool * A) :=
+  match n with
+  | O => OutOfFuel
+  | S n =>
+      if (is_value t) then Result (true, t)
+      else match step m t with
+           | Some t => multistep' m n step t is_value
+           | None => Result ((is_value t), t)
+           end
+  end.
+
