theories/QCLibs.v
@@ -1,5 +1,18 @@
-From Coq Require Export Arith Lia List String Program.Wf.
-From Coq Require Export Recdef.
+From Coq Require Export
+     Arith Lia List String Program.Wf Program.Equality.
+From Coq Require Export
+     Recdef ssreflect ssrfun ssrbool.
 From QuickChick Require Export QuickChick.
 From ExtLib Require Export Monad OptionMonad ListMonad.
 Export QcNotation MonadNotation ListNotations.
+
+(* Set Implicit Arguments. *)
+(* Unset Strict Implicit. *)
+(* Unset Printing Implicit Defensive. *)
+
+Ltac inv0 :=
+  let H := fresh "H" in
+  intros H; inversion H; clear H; subst.
+
+Ltac inv H :=
+  inversion H; clear H; subst.
