theories/ReductionM.v
@@ -1,0 +1,107 @@
+From FSUB Require Import QCLibs.
+From FSUB Require Import FSub.
+From FSUB Require Import Decidable.
+
+(** ** Computable Reduction Semantics *)
+Program Definition ctx_inj (t : term) : option (ctx * term) :=
+  match t with
+  | app t1 t2 =>
+      match dc_value t1 with
+        true => Some (@c_apparg t1 _ c_hole, t2)
+      | false => Some (c_appfun c_hole t2, t1)
+      end
+  | tapp t1 T2 =>
+      Some (c_typefun c_hole T2,  t1)
+  | _ => None
+  end.
+Next Obligation.
+  apply dc_value_implies_value. auto.
+Qed.
+Solve All Obligations with easy.
+
+Eval cbn in (ctx_inj (tapp (var 0) top)).
+
+Fixpoint measure_term (t : term) : nat :=
+  match t with
+  | var _ => 1 
+  | abs _ t' => 1 + measure_term t'
+  | app t1 t2 => 1 + measure_term t1 + measure_term t2
+  | tabs _ t2 => 1 + measure_term t2
+  | tapp t1 _ => 1 + measure_term t1
+  end.
+
+Lemma measure_term_le_ctx_inj : forall c t t',
+    Some (c, t') = ctx_inj t -> measure_term t' < measure_term t.
+Proof.
+  intros until t. destruct t; intros; cbn in *; try congruence. 
+  - destruct t1; cbn in *; inversion H; clear H; subst; cbn; lia.
+  - inversion H; clear H; subst; lia. 
+Qed.
+
+Program Fixpoint step (t : term) {measure (measure_term t)} : option term :=
+  match t with
+  | app (abs _ t12) t2 =>
+      if dc_value t2 then Some (subst t12 0 t2) else
+        match ctx_inj t with
+        | None => None
+        | Some (c', t') => 
+            match step t' with
+            | Some t'' => Some (ctx_app c' t'')
+            | None => None
+            end
+        end         
+  | tapp (tabs T11 t12) T2 => Some (subst_typ t12 0 T2)
+  | _ => match ctx_inj t with
+         | None => None
+         | Some (c', t') => 
+             match step t' with
+             | Some t'' => Some (ctx_app c' t'')
+             | None => None
+             end
+         end 
+  end.
+Next Obligation.
+  cbn; lia.
+Qed.
+Next Obligation.
+  eapply measure_term_le_ctx_inj. eauto.
+Qed.
+Solve All Obligations with easy.
+
+Compute (step (app
+                 (abs top (var 0))
+                 (abs top (var 0)))).
+Compute (step (abs top (var 0))).
+
+(* Require Extraction. *)
+(* Extraction "step.ml" step. *)
+
+Lemma step_app_value : forall T t1 t2,
+    dc_value t2 = true -> step (app (abs T t1) t2) = Some (subst t1 0 t2).
+Proof.
+Admitted.  
+
+(** ** Equivalence in Reduction Semantics *)
+Lemma step_is_red : forall t t', step t = Some t' -> red t t'.
+Proof with intuition. 
+  induction t; intros t'; simpl; intros.
+  - cbn in H; congruence.
+  - cbn in H; congruence.
+  - destruct t1.
+    + cbn in H. congruence.
+    + destruct (dc_value t2) eqn:Et2.
+      * pose proof Et2 as Et2'.
+        apply dc_value_implies_value in Et2.
+        rewrite step_app_value in H. inversion H; subst. constructor.
+        assumption.
+        assumption.
+Admitted.
+
+Lemma red_is_step : forall t t', red t t' -> step t = Some t'.
+Admitted.
+    
+Lemma red_iff_step : forall t t', red t t' <-> step t = Some t'.
+Proof.
+  split. apply red_is_step. apply step_is_red.
+Qed.
+
